tests/fstar/hashmap/Hashmap.Clauses.fst
@@ -8,54 +8,54 @@ open Hashmap.Types
 
 (** [hashmap::HashMap::allocate_slots]: decreases clause *)
 unfold
-let hash_map_allocate_slots_decreases (t : Type0) (slots : vec (list_t t))
+let hash_map_allocate_slots_loop_decreases (t : Type0) (slots : vec (list_t t))
   (n : usize) : nat = n
 
 (** [hashmap::HashMap::clear_slots]: decreases clause *)
 unfold
-let hash_map_clear_slots_decreases (t : Type0) (slots : vec (list_t t))
+let hash_map_clear_slots_loop_decreases (t : Type0) (slots : vec (list_t t))
   (i : usize) : nat =
   if i < length slots then length slots - i else 0
 
 (** [hashmap::HashMap::insert_in_list]: decreases clause *)
 unfold
-let hash_map_insert_in_list_decreases (t : Type0) (key : usize) (value : t)
+let hash_map_insert_in_list_loop_decreases (t : Type0) (key : usize) (value : t)
   (ls : list_t t) : list_t t =
   ls
 
 (** [hashmap::HashMap::move_elements_from_list]: decreases clause *)
 unfold
-let hash_map_move_elements_from_list_decreases (t : Type0)
+let hash_map_move_elements_from_list_loop_decreases (t : Type0)
   (ntable : hash_map_t t) (ls : list_t t) : list_t t =
   ls
 
 (** [hashmap::HashMap::move_elements]: decreases clause *)
 unfold
-let hash_map_move_elements_decreases (t : Type0) (ntable : hash_map_t t)
+let hash_map_move_elements_loop_decreases (t : Type0) (ntable : hash_map_t t)
   (slots : vec (list_t t)) (i : usize) : nat =
   if i < length slots then length slots - i else 0
 
 (** [hashmap::HashMap::contains_key_in_list]: decreases clause *)
 unfold
-let hash_map_contains_key_in_list_decreases (t : Type0) (key : usize)
+let hash_map_contains_key_in_list_loop_decreases (t : Type0) (key : usize)
   (ls : list_t t) : list_t t =
   ls
 
 (** [hashmap::HashMap::get_in_list]: decreases clause *)
 unfold
-let hash_map_get_in_list_decreases (t : Type0) (key : usize) (ls : list_t t) :
+let hash_map_get_in_list_loop_decreases (t : Type0) (key : usize) (ls : list_t t) :
   list_t t =
   ls
 
 (** [hashmap::HashMap::get_mut_in_list]: decreases clause *)
 unfold
-let hash_map_get_mut_in_list_decreases (t : Type0) (ls : list_t t)
+let hash_map_get_mut_in_list_loop_decreases (t : Type0) (ls : list_t t)
   (key : usize) : list_t t =
   ls
 
 (** [hashmap::HashMap::remove_from_list]: decreases clause *)
 unfold
-let hash_map_remove_from_list_decreases (t : Type0) (key : usize)
+let hash_map_remove_from_list_loop_decreases (t : Type0) (key : usize)
   (ls : list_t t) : list_t t =
   ls
 
